examples/mem/MemMemClient.v
@@ -1,0 +1,221 @@
+Require Import Coqlib.
+Require Import ITreelib.
+Require Import Universe.
+Require Import STS.
+Require Import Behavior.
+Require Import ModSem.
+Require Import Skeleton.
+Require Import PCM.
+Require Import Hoare Open OpenDef.
+Require Import SimModSem Weakening.
+
+Set Implicit Arguments.
+
+
+
+Require Import Mem0 Mem1 MemOpen Mem0Openproof MemClient0 MemClient1 MemClient01proof.
+
+
+
+
+
+Arguments rel_dec_eq_true [T] eqt {r} {rc}.
+(* rel_dec_eq_true =  *)
+(* fun (T : Type) (eqt : T -> T -> Prop) (r : RelDec eqt) (rc : RelDec_Correct r) *)
+(*   (x y : T) (H : eqt x y) => *)
+(* let H0 : forall x0 y0 : T, eqt x0 y0 -> x0 ?[ eqt ] y0 = true := *)
+(*   fun x0 y0 : T => match rel_dec_correct x0 y0 with *)
+(*                    | conj _ x2 => x2 *)
+(*                    end in *)
+(* let H1 : x ?[ eqt ] y = true := H0 x y H in H1 *)
+(*      : forall (T : Type) (eqt : T -> T -> Prop) (r : RelDec eqt), *)
+(*        RelDec_Correct r -> forall x y : T, eqt x y -> x ?[ eqt ] y = true *)
+
+(* Arguments rel_dec_eq_true [T]%type_scope [eqt]%function_scope [r] _ _ _ _ *)
+
+
+Section WEAKENINGAUX.
+  Context `{Σ: GRA.t}.
+
+  Definition stb_le (stb0 stb1: list (string * fspec)) :=
+    forall fn fsp0 (FINDTGT: alist_find fn stb0 = Some (fsp0)),
+    exists fsp1,
+      (<<FINDSRC: alist_find fn stb1 = Some (fsp1)>>) /\
+      (<<WEAKER: fspec_weaker fsp0 fsp1>>)
+  .
+
+  Variable md: (Sk.t -> list (string * fspec)) -> Mod.t.
+  Variable _stb0 _stb1: (Sk.t -> list (string * fspec)).
+  Hypothesis WEAKEN: forall sk, stb_le (_stb0 sk) (_stb1 sk).
+
+  Theorem adequacy_weaken
+          sk
+    :
+      <<SIM: ModSemPair.sim (Mod.get_modsem (md _stb0) sk) (Mod.get_modsem (md _stb1) sk)>>
+  .
+  Proof.
+    TTTTTTTTTTTTTTTTTTTTTTTTTTTT
+  Qed.
+
+End WEAKENINGAUX.
+
+Section WEAKENING.
+
+  Context `{Σ: GRA.t}.
+  Context `{@GRA.inG memRA Σ}.
+
+  Require Import Logic TODOYJ.
+
+
+  Let weaken: forall (fn : string) (fsp_tgt : fspec),
+      alist_find fn MemStb = Some fsp_tgt ->
+      exists (fsp_src : fspec),
+        (<< _ : alist_find fn (MemStb ++ ClientStb) = Some fsp_src >>) /\ << _ : fspec_weaker fsp_tgt fsp_src >>
+  .
+  Proof.
+    ii. stb_tac. des_ifs.
+    - rewrite eq_rel_dec_correct in *. des_ifs. subst. esplits; eauto. { stb_tac. ss. } refl.
+    - rewrite eq_rel_dec_correct in *. des_ifs. subst. esplits; eauto. { stb_tac. ss. } refl.
+    - rewrite eq_rel_dec_correct in *. des_ifs. subst. esplits; eauto. { stb_tac. ss. } refl.
+    - rewrite eq_rel_dec_correct in *. des_ifs. subst. esplits; eauto. { stb_tac. ss. } refl.
+    - rewrite eq_rel_dec_correct in *. des_ifs. subst. esplits; eauto. { stb_tac. ss. } refl.
+  Qed.
+
+End WEAKENING.
+
+
+
+
+
+Section AUX.
+
+  Theorem GRA_wf_embed
+          A
+          `{@GRA.inG A Σ}
+          (a: A)
+          (WF: URA.wf a)
+    :
+      URA.wf (GRA.embed a)
+  .
+  Proof.
+    ss. ii. unfold GRA.embed.
+    Local Transparent GRA.to_URA. ur. i. des_ifs; cycle 1.
+    { apply URA.wf_unit. }
+    ss. unfold PCM.GRA.cast_ra, eq_rect, eq_sym. destruct GRA.inG_prf. ss.
+    Local Opaque GRA.to_URA.
+  Qed.
+
+  Theorem Auth_wf_black
+          `{M: URA.t}
+          a
+          (WF: URA.wf a)
+    :
+      <<WF: URA.wf (Auth.black a)>>
+  .
+  Proof. ur. split; ss. r. esplits. rewrite URA.unit_idl. refl. Qed.
+
+End AUX.
+
+
+
+Require Import Open.
+
+Section PROOF.
+
+  Context `{Σ: GRA.t}.
+  Context `{@GRA.inG memRA Σ}.
+
+  Variable _ctxs: list UMod.t.
+  Let ctxs := List.map UMod.to_mod _ctxs.
+
+  Let global_stb sk :=
+    MemStb ++ ClientStb ++
+    flat_map (map (map_snd (λ _, fspec_trivial2)) ∘ UModSem.fnsems) (map (flip UMod.get_modsem sk) _ctxs).
+
+  Definition MemClient0 := Mod.add_list ([Mem0.Mem; MemClient0.Client] ++ ctxs).
+  Definition MemClient1 :=
+    Mod.add_list ([MemOpen.Mem (fun _ => []);
+                  MemClient1.Client (fun _ => (UnknownStb ++ ClientStb ++ MemStb))] ++ ctxs).
+  Definition MemClient2 := Mod.add_list ([MemOpen.Mem global_stb; MemClient1.Client global_stb] ++ ctxs).
+  Definition MemClient3 := Mod.add_list ([KMod.to_src MemOpen.KMem; KMod.to_src MemClient1.KClient] ++ ctxs).
+
+  Let TODO_REMOVE_THIS: SimModSem.ModPair.sim (MemOpen.Mem (fun _ => [])) Mem0.Mem.
+  Proof.
+    econs.
+    { ii. eapply SimModSem.adequacy_lift.
+      replace (Mod.get_modsem Mem0.Mem sk) with (Mem0.MemSem sk) by refl.
+      replace (Mod.get_modsem (MemOpen.Mem (fun _ => [])) sk) with (MemOpen.MemSem [] sk) by refl.
+      eapply Mem0Openproof.correct.
+    }
+    { ss. }
+    { ii. repeat (econs; ss; ii; des; ss). }
+  Qed.
+
+  Let correct01: refines_closed MemClient0 MemClient1.
+  Proof.
+    etrans; cycle 1.
+    { instantiate (1:=Mod.add_list ([Mem0.Mem; MemClient1.Client (fun _ => (UnknownStb ++ ClientStb ++ MemStb))] ++ ctxs)).
+      eapply refines_close.
+      unfold MemClient1. rewrite ! Mod.add_list_app. eapply (SimModSem.refines_proper_r).
+      hexploit (SimModSem.refines_proper_r [MemOpen.Mem (fun _ => [])] [Mem0.Mem]
+                                           [MemClient1.Client (fun _ => (UnknownStb ++ ClientStb ++ MemStb))]).
+      { cbn. rewrite ! ModL.add_empty_r. eapply SimModSem.adequacy_local. eapply TODO_REMOVE_THIS. }
+      intro T; des. cbn in T. rewrite ! ModL.add_empty_r in T. ss.
+    }
+    etrans; cycle 1.
+    { instantiate (1:=Mod.add_list ([Mem0.Mem; MemClient0.Client] ++ ctxs)).
+      eapply refines_close.
+      rewrite ! Mod.add_list_app. eapply (SimModSem.refines_proper_r).
+      hexploit (SimModSem.refines_proper_l [MemClient1.Client (fun _ => (UnknownStb ++ ClientStb ++ MemStb))]
+                                           [MemClient0.Client] [Mem0.Mem]).
+      { cbn. rewrite ! ModL.add_empty_r. eapply SimModSem.adequacy_local.
+        eapply MemClient01proof.correct.
+      }
+      intro T; des. cbn in T. rewrite ! ModL.add_empty_r in T. ss.
+    }
+    refl.
+  Qed.
+
+  Let mem_sbtb_stb: (MemStb) = (List.map (map_snd (fun ksb => (KModSem.disclose_ksb ksb): fspec)) (MemSbtb)).
+  Proof. ss. unfold MemStb. unseal "stb". refl. Qed.
+
+  Let client_sbtb_stb:
+    (ClientStb) = (List.map (map_snd (fun ksb => (KModSem.disclose_ksb ksb): fspec)) (ClientSbtb)).
+  Proof. ss. unfold ClientStb. unseal "stb". refl. Qed.
+
+  Let _kmds: list KMod.t := [KMem; KClient].
+
+  Lemma map_snd_map_snd A B0 B1 B2 (f0: B0 -> B1) (f1: B1 -> B2):
+    (map_snd (A:=A) f1) ∘ (map_snd f0) = map_snd (f1 ∘ f0).
+  Proof. apply func_ext. i. destruct x; ss. Qed.
+
+  Let correct12: refines_closed MemClient1 MemClient2.
+  Proof.
+  Qed.
+
+  Let correct23: refines_closed MemClient2 MemClient3.
+  Proof.
+    rp; [eapply (adequacy_open _kmds _ctxs)|..]; revgoals.
+    { refl. }
+    { unfold MemClient1.
+      fold ctxs.
+      remember _kmds. repeat f_equal. subst.
+      unfold _kmds. Opaque MemSbtb. Opaque ClientSbtb. cbn.
+      unfold Mem, Client.
+      replace (λ ske : Sk.t,
+       (map (map_snd fsb_fspec) (map (map_snd KModSem.disclose_ksb) MemSbtb) ++
+        map (map_snd fsb_fspec) (map (map_snd KModSem.disclose_ksb) ClientSbtb) ++ []) ++
+       flat_map
+         (map (map_snd (λ _ : list val → itree (uCallE +' pE +' eventE) val, fspec_trivial2)) ∘ UModSem.fnsems)
+         (map (flip UMod.get_modsem ske) _ctxs)) with
+          global_stb; cycle 1.
+      { apply func_ext. intro sk. rewrite app_nil_r.
+        unfold global_stb.
+        rewrite ! map_map. rewrite ! map_snd_map_snd.
+        rewrite <- mem_sbtb_stb.
+        rewrite <- client_sbtb_stb. rewrite <- List.app_assoc. repeat f_equal. }
+      f_equal.
+    }
+  Qed.
+
+End PROOF.
